Maybe using match in types?

WfInduct/Basic.lean
@@ -81,8 +81,7 @@ partial def foldCalls (fn : Expr) (oldIH : FVarId) (e : Expr) : MetaM Expr := do
 -- (TODO: Worth folding with `foldCalls`, like before?)
 -- (TODO: Accumulated with a left fold)
 -- (TODO: Revert context in the leaf, based on local context?)
-partial def collectIHs (fn : Expr) (oldIH newIH : FVarId) (e : Expr) :
-    MetaM (Array Expr) := do
+partial def collectIHs (fn : Expr) (oldIH newIH : FVarId) (e : Expr) : MetaM (Array Expr) := do
   if ! e.hasAnyFVar (· == oldIH) then
     return #[]
   else if e.getAppNumArgs = 2 && e.getAppFn.isFVarOf oldIH then
@@ -108,11 +107,10 @@ partial def collectIHs (fn : Expr) (oldIH newIH : FVarId) (e : Expr) :
       let ihs2 ← collectIHs fn oldIH newIH (b.instantiate1 x)
       let ihs2 ← ihs2.mapM (mkLetFun x v' ·)
       return ihs1 ++ ihs2
-  /- This is tricky! Not sure what best to do here.
-  if let some matcherApp ← matchMatcherApp? e then
+  else if let some matcherApp ← matchMatcherApp? e then
     -- logInfo m!"{matcherApp.matcherName} {goal} {←inferType (Expr.fvar newIH)} => {matcherApp.discrs} {matcherApp.remaining}"
     if matcherApp.remaining.size == 1 && matcherApp.remaining[0]!.isFVarOf oldIH then
-      let motive' ← lambdaTelescope matcherApp.motive fun motiveArgs _motiveBody => do
+      let (motive', goalMVar) ← lambdaTelescope matcherApp.motive fun motiveArgs _motiveBody => do
         unless motiveArgs.size == matcherApp.discrs.size do
           throwError "unexpected matcher application, motive must be lambda expression with #{matcherApp.discrs.size} arguments"
 
@@ -124,14 +122,10 @@ partial def collectIHs (fn : Expr) (oldIH newIH : FVarId) (e : Expr) :
           let eTypeAbst ← kabstract eTypeAbst discr
           return eTypeAbst.instantiate1 motiveArg
 
-        let goalAbst ← matcherApp.discrs.size.foldRevM (init := goal) fun i goalAbst => do
-          let motiveArg := motiveArgs[i]!
-          let discr     := matcherApp.discrs[i]!
-          let goalAbst ← kabstract goalAbst discr
-          return goalAbst.instantiate1 motiveArg
+        let goalMVar ← mkFreshExprSyntheticOpaqueMVar (.sort levelZero) (tag := `goal)
 
-        let motiveBody ← mkArrow eTypeAbst goalAbst
-        mkLambdaFVars motiveArgs motiveBody
+        let motiveBody ← mkArrow eTypeAbst goalMVar
+        return (← mkLambdaFVars motiveArgs motiveBody, goalMVar)
 
       let matcherLevels ← match matcherApp.uElimPos? with
         | none     => pure matcherApp.matcherLevels
@@ -147,32 +141,51 @@ partial def collectIHs (fn : Expr) (oldIH newIH : FVarId) (e : Expr) :
         throwError "failed to add argument to matcher application, type error when constructing the new motive"
       let mut auxType ← inferType aux
 
-      let mut altIHss := #[]
+      let mut altIHs : Array Expr := #[]
       for alt in matcherApp.alts,
           numParams in matcherApp.altNumParams do
         let Expr.forallE _ d b _ ← whnfD auxType | unreachable!
-        let altIHs ← forallBoundedTelescope d (some numParams) fun xs d => do
+        let altIH ← forallBoundedTelescope d (some numParams) fun xs d => do
           let alt ← try instantiateLambda alt xs[:numParams] catch _ => throwError "unexpected matcher application, insufficient number of parameters in alternative"
-          let altIHs ← removeLamda alt fun oldIH' alt => do
-            let altIHs ← forallBoundedTelescope d (some 1) fun newIH' goal' => do
+          let altIH ← removeLamda alt fun oldIH' alt => do
+            forallBoundedTelescope d (some 1) fun newIH' _goal' => do
               let #[newIH'] := newIH' | unreachable!
-              -- logInfo m!"goal': {goal'}"
-              let alsIHs ← collectIHs fn oldIH' newIH'.fvarId! alt
-              altIHs.mapM (mkLambdaFVars #[newIH'])
-            altIHs.mapM (mkLambdaFVars xs)
+              let altIHs ← collectIHs fn oldIH' newIH'.fvarId! alt
+              let altIH := altIHs.foldr (mkApp2 (.const ``And.intro [])) (.const ``True.intro [])
+              mkLambdaFVars #[newIH'] altIH
+          mkLambdaFVars xs altIH
         let dummy := mkSort levelZero
         auxType := b.instantiate1 dummy -- ugh, what to instantiate here? Lets hope they are unused
-        altIHss := altIHss.push altIHs
+        altIHs := altIHs.push altIH
+
+      -- Now figure out the type, with an explicit match
+      let propMotive ← lambdaTelescope motive' fun motiveArgs _motiveBody => do
+        mkLambdaFVars motiveArgs (.sort levelZero)
+      let propAlts ← altIHs.mapM fun altIH =>
+        lambdaTelescope altIH fun xs altIH => do
+          logInfo "Foo"
+          mkForallFVars xs (← inferType altIH)
+      let typeMatcherApp := { matcherApp with
+        motive := propMotive
+        alts := propAlts
+        remaining     := #[] -- matcherApp.remaining.set! 0 (.fvar newIH)
+      }
+      goalMVar.mvarId!.assign typeMatcherApp.toExpr
+      logInfo m!"Bar: {← instantiateMVars goalMVar}"
+      check (← instantiateMVars goalMVar)
+      logInfo "Baz"
+
       let matcherApp' := { matcherApp with
         matcherLevels := matcherLevels,
         motive        := motive',
-        alts          := alts',
+        alts          := altIHs,
         remaining     := matcherApp.remaining.set! 0 (.fvar newIH)
       }
       -- check matcherApp'.toExpr
       -- logInfo m!"matcherApp' {matcherApp'.toExpr}"
-      return matcherApp'.toExpr
-  -/
+      return #[ matcherApp'.toExpr ]
+    else
+      throwError "collectIHs: non-refining matcher?"
   else if e.getAppArgs.any (·.isFVarOf oldIH) then
     throwError "collectIHs: could not collect recursive calls from {indentExpr e}"
   else if let .app e1 e2 := e then
@@ -605,3 +618,31 @@ elab "#derive_induction " ident:ident : command => runTermElabM fun _xs => do
   let [name] ← resolveGlobalConst ident
     | throwErrorAt ident m!"ambiguous identifier"
   deriveInduction name
+
+
+def match_non_tail (n : Nat ) : Bool :=
+  n = 42 || match n with
+  | 0 => true
+  | n+1 => match_non_tail n
+termination_by n
+
+def match_non_tail_induct
+  {motive : Nat → Prop}
+  (case1 : forall n, (IH : match n with | 0 => True | n+1 => motive n) → motive n)
+  (n : Nat) : motive n :=
+  WellFounded.fix Nat.lt_wfRel.wf (fun n IH =>
+    match n with
+    | 0 => case1 0 True.intro
+    | n+1 =>
+      case1 (n+1) (IH n (Nat.lt_succ_self _))
+  ) n
+
+theorem match_non_tail_eq_true (n : Nat) : match_non_tail n = true := by
+  induction n using match_non_tail_induct
+  case case1 n IH =>
+    unfold match_non_tail
+    split <;> dsimp at IH <;> simp [IH]
+
+
+set_option pp.rawOnError true in
+#derive_induction match_non_tail
